#################################################################
# Catena-X "Diagnosis" Domain Ontology in TTL/RDF/OWL FORMAT
# See copyright notice in the top folder
# See authors file in the top folder
# See license file in the top folder
#################################################################

@prefix : <https://github.com/catenax-ng/product-knowledge/ontology/diagnosis.ttl#> .
@prefix cx: <https://github.com/catenax-ng/product-knowledge/ontology/cx.ttl#> .
@prefix cx-diag: <https://github.com/catenax-ng/product-knowledge/ontology/diagnosis.ttl#> .
@prefix owl: <http://www.w3.org/2002/07/owl#> .
@prefix rdf: <http://www.w3.org/1999/02/22-rdf-syntax-ns#> .
@prefix xml: <http://www.w3.org/XML/1998/namespace> .
@prefix xsd: <http://www.w3.org/2001/XMLSchema#> .
@prefix rdfs: <http://www.w3.org/2000/01/rdf-schema#> .
@prefix dcterms: <http://purl.org/dc/terms/> .
@base <https://github.com/catenax-ng/product-knowledge/ontology/diagnosis.ttl#> .

cx-diag: rdf:type owl:Ontology ;
    dcterms:description "The Catena-X Diagnosis Domain describes knowledge about automotive (electronic) diagnosis processes."@en ;
    dcterms:title "Catena-X Diagnosis Domain" ;
    owl:versionInfo "0.5.1" .

cx-diag:DTC rdf:type owl:Class ;
    dcterms:description "A Diagnostic Trouble Code (DTC) is a (BusinessPartner-specific) trouble condition that is (either directly or in parts) indicated through an electronic diagnosis."@en ;
    dcterms:title "Diagnostic Trouble Code" ;
    rdfs:subClassOf cx:Asset .

cx-diag:Code rdf:type owl:DatatypeProperty ;
    dcterms:description "The Code of a Diagnostic Trouble Code (DTC) is a (BusinessPartner-specific) identifier that is shown in protocols."@en ;
    dcterms:title "DTC Code" ;
    rdfs:domain cx-diag:DTC ;
    rdfs:range xsd:string .

cx-diag:Description rdf:type owl:DatatypeProperty ;
    dcterms:description "The Description of a Diagnostic Trouble Code (DTC) is an interationalized paragraph/sentence describing a trouble condition."@en ;
    dcterms:description "Deutsche Beschreibung."@de ;
    dcterms:title "DTC Description" ;
    rdfs:domain cx-diag:DTC ;
    rdfs:range xsd:string .

cx-diag:PossibleCauses rdf:type owl:DatatypeProperty ;
    dcterms:description "The Possible Causes of a Diagnostic Trouble Code (DTC) are identifiers to possible root causes of a trouble condition."@en ;
    dcterms:title "DTC Possible Causes" ;
    rdfs:domain cx-diag:DTC ;
    rdfs:range xsd:string .

cx-diag:Version rdf:type owl:DatatypeProperty ;
    dcterms:description "The Version of a Diagnostic Trouble Code (DTC) describes the version of the condition in the Business Partners DTC catalogue."@en ;
    dcterms:title "DTC Version" ;
    rdfs:domain cx-diag:DTC ;
    rdfs:range xsd:long .

cx-diag:DiagnosedPart rdf:type owl:Class ;
    dcterms:description "A Diagnosed Part describes any aggregate/component that is observed to an electronic diagnosis."@en ;
    dcterms:title "Diagnosed Part" ;
    rdfs:subClassOf cx:Asset .

cx-diag:EnDenomination rdf:type owl:DatatypeProperty ;
    dcterms:description "The EnDenomination of a Diagnosed Part is an internationalized unique name."@en ;
    dcterms:title "Diagnosed Part EnDenomination" ;
    rdfs:domain cx-diag:DiagnosedPart ;
    rdfs:range xsd:string .

cx-diag:Classification rdf:type owl:DatatypeProperty ;
    dcterms:description "The Classification of a Diagnosed Part is what?."@en ;
    dcterms:title "Diagnosed Part Classification" ;
    rdfs:domain cx-diag:DiagnosedPart ;
    rdfs:range xsd:string .

cx-diag:Category rdf:type owl:DatatypeProperty ;
    dcterms:description "The Category of a Diagnosed Part categorizes the part in a hierarchy."@en ;
    dcterms:title "Diagnosed Part Category" ;
    rdfs:domain cx-diag:DiagnosedPart ;
    rdfs:range xsd:string .

cx-diag:affects rdf:type owl:ObjectProperty ;
    dcterms:description "The affects predicate connects Diagnostic Trouble Codes (DTC) with the diagnosed parts."@en ;
    dcterms:title "Affects" ;
    rdfs:domain cx-diag:DTC ;
    rdfs:range cx-diag:DiagnosedPart .

###  Generated by the OWL API (version 4.5.9.2019-02-01T07:24:44Z) https://github.com/owlcs/owlapi
