@prefix : <https://w3id.org/catenax/ontology/vfunction#> .
@prefix dc: <http://purl.org/dc/elements/1.1/> .
@prefix owl: <http://www.w3.org/2002/07/owl#> .
@prefix rdf: <http://www.w3.org/1999/02/22-rdf-syntax-ns#> .
@prefix xml: <http://www.w3.org/XML/1998/namespace> .
@prefix xsd: <http://www.w3.org/2001/XMLSchema#> .
@prefix rdfs: <http://www.w3.org/2000/01/rdf-schema#> .
@prefix skos: <http://www.w3.org/2004/02/skos/core#> .
@prefix schema: <https://schema.org/> .
@prefix cx-common: <https://w3id.org/catenax/ontology/common#> .
@prefix cx-fx: <https://w3id.org/catenax/ontology/function#> .
@base <https://w3id.org/catenax/ontology/function> .

<https://w3id.org/catenax/ontology/function> rdf:type owl:Ontology ;
                                             dc:contributor "Oguzhan Balandi" ;
                                             dc:creator "Christoph Jung" ;
                                             dc:date "2023-06-29"^^xsd:date ;
                                             dc:description "Ontology for function invocations." ;
                                             dc:title "Function Ontology" ;
                                             owl:imports <file:common_ontology.ttl>;
                                             owl:versionInfo "1.9.4" .

###  https://w3id.org/catenax/ontology/function#Function
cx-fx:Function rdf:type owl:Class ;
               rdfs:subClassOf cx-core:ConceptualObject ;
               skos:altLabel "Function Definition"@en ;
               skos:prefLabel "Function"@en .

###  https://w3id.org/catenax/ontology/function#callbackAddress
cx-fx:callbackAddress rdf:type owl:ObjectProperty ;
                              rdfs:domain rdfs:Resource;
                              rdfs:range rdfs:Resource;
                              skos:example <http://localhost:8888/callback>;
                              rdfs:comment  "Documents that a given resource exhibits a callback endpoint. The URI/IRI should resolve to some existing URL."@en ;
                              skos:prefLabel "Callback Address"@en .

###  https://w3id.org/catenax/ontology/function#supportsInvocation
cx-fx:supportsInvocation rdf:type owl:ObjectProperty ;
                              rdfs:domain rdfs:Resource;
                              rdfs:range cx-fx:Function;
                              skos:note "Documents that a given resource supports a certain function."@en ;
                              skos:prefLabel "Function Support"@en .

###  https://w3id.org/catenax/ontology/function#targetUri
cx-fx:targetUri rdf:type owl:ObjectProperty ;
                              rdfs:domain cx-fx:Function ;
                              rdfs:range rdfs:Resource;
                              skos:example <class:org.eclipse.tractusx.agents.remoting.TestFunction#test> ;
                              skos:example <http://tiera-backend:5005/api/rul> ;
                              skos:example <https://api.agify.io> ;
                              rdfs:comment  "The target URI of the function should resolve to some existing service (URL)."@en ;
                              skos:prefLabel "Target URI"@en .

###  https://w3id.org/catenax/ontology/function#invocationMethod
cx-fx:invocationMethod rdf:type owl:DatatypeProperty ;
              rdfs:comment "Determines the invocation method of the function in case that the target service provides several possibilities."@en;
              rdfs:subPropertyOf owl:topDataProperty ;
              rdfs:domain cx-fx:Function ;
              rdfs:range xsd:string;
              skos:example "DEFAULT";
              skos:example "GET";
              skos:example "POST-JSON-MF";
              skos:example "POST-JSON";
              skos:example "POST-XML-MF";
              skos:example "POST-XML";
              skos:prefLabel "Invocation Method"@en .

###  https://w3id.org/catenax/ontology/function#batch
cx-fx:batch rdf:type owl:DatatypeProperty ;
            rdfs:comment "Determines maximal batch size for function invocations. Default is '1' which means that each invocation is done separately"@en;
            rdfs:subPropertyOf owl:topDataProperty ;
            rdfs:domain cx-fx:Function ;
            rdfs:range xsd:long;
            skos:example "100"^^xsd:long;
            skos:altLabel "Maximal Batch Size"@en;
            skos:prefLabel "Batch Size"@en .

###  https://w3id.org/catenax/ontology/function#inputProperty
cx-fx:inputProperty rdf:type owl:DatatypeProperty ;
            rdfs:comment "Determines a path/name in the input document under which all input arguments are encoded. Default is '.'"@en;
            rdfs:subPropertyOf owl:topDataProperty ;
            rdfs:domain cx-fx:Function ;
            rdfs:range xsd:string;
            skos:example ".";
            skos:altLabel "Function Input Property"@en;
            skos:prefLabel "Input Property"@en .

###  https://w3id.org/catenax/ontology/function#invocationIdProperty
cx-fx:invocationIdProperty rdf:type owl:DatatypeProperty ;
            rdfs:comment "Determines a (set of) paths in the input document under which the IRI of the invocation (instance of Function) will be transmitted."@en;
            rdfs:subPropertyOf owl:topDataProperty ;
            rdfs:domain cx-fx:Function ;
            rdfs:range xsd:string;
            skos:example "requestId";
            skos:altLabel "Function Invocation ID Property"@en;
            skos:prefLabel "Invocation ID Property"@en .

###  https://w3id.org/catenax/ontology/function#callbackProperty
cx-fx:callbackProperty rdf:type owl:DatatypeProperty ;
            rdfs:comment "Determines a (set of) paths in the input document and the output response under which the callback address (see <https://w3id.org/catenax/ontology/function#callbackAddress>) and the referring callback id will be transmitted."@en;
            rdfs:subPropertyOf owl:topDataProperty ;
            rdfs:domain cx-fx:Function ;
            rdfs:domain cx-fx:Result ;
            rdfs:range xsd:string;
            skos:example "callbackAddress";
            skos:altLabel "Function Callback ID/Address Property"@en;
            skos:prefLabel "Callback Address"@en .

###  https://w3id.org/catenax/ontology/function#input
cx-fx:input rdf:type owl:ObjectProperty ;
            rdfs:domain cx-fx:Function ;
            rdfs:range cx-fx:Argument;
            rdfs:comment  "Describes the arguments of a function."@en ;
            skos:prefLabel "Input Argument"@en .

###  https://w3id.org/catenax/ontology/function#input
cx-fx:result rdf:type owl:ObjectProperty ;
            rdfs:domain cx-fx:Function ;
            rdfs:range cx-fx:Result;
            rdfs:comment  "Describes the result of a function."@en ;
            skos:prefLabel "Output Result"@en .

###  https://w3id.org/catenax/ontology/function#Argument
cx-fx:Argument rdf:type owl:Class ;
               rdfs:subClassOf cx-core:ConceptualObject ;
               skos:altLabel "Function Argument Definition"@en ;
               skos:prefLabel "Argument"@en .

###  https://w3id.org/catenax/ontology/function#Result
cx-fx:Result rdf:type owl:Class ;
             rdfs:subClassOf cx-core:ConceptualObject ;
             skos:altLabel "Function Result Definition"@en ;
             skos:prefLabel "Result"@en .


###  https://w3id.org/catenax/ontology/function#argumentName
cx-fx:argumentName rdf:type owl:DatatypeProperty ;
            rdfs:comment "Determines the name or index of the function argument.";
            rdfs:subPropertyOf owl:topDataProperty ;
            rdfs:domain cx-fx:Argument ;
            rdfs:range xsd:string;
            skos:example "arg0";
            skos:example "age";
            skos:altLabel "Argument Name or Index"@en;
            skos:prefLabel "Argument Name"@en .

###  https://w3id.org/catenax/ontology/function#argumentName
cx-fx:dataType rdf:type owl:DatatypeProperty ;
               rdfs:comment "Determines the data type of an argument or return value.";
               rdfs:subPropertyOf owl:topDataProperty ;
               rdfs:domain cx-fx:Argument;
               rdfs:domain cx-fx:ReturnValue ];
               rdfs:range rdfs:Datatype;
               skos:example json:Object;
               skos:example xsd:long;
               skos:altLabel "Argument or Result Data Type"@en;
               skos:prefLabel "Argument or Result Data Type"@en .

###  https://w3id.org/catenax/ontology/function#priority
cx-fx:priority rdf:type owl:DatatypeProperty ;
            rdfs:comment "Determines the priority with which the argument is processed. Default is '10'"@en;
            rdfs:subPropertyOf owl:topDataProperty ;
            rdfs:domain cx-fx:Argument ;
            rdfs:range xsd:integer;
            skos:example "-1"^^xsd:integer;
            skos:altLabel "Argument Priority"@en;
            skos:prefLabel "Priority"@en .

###  https://w3id.org/catenax/ontology/function#default
cx-fx:default rdf:type owl:DatatypeProperty ;
            rdfs:comment "Determines a default for the given argument which is taken if this is a mandatory argument (see <https://w3id.org/catenax/ontology/function#mandatory>)"@en;
            rdfs:subPropertyOf owl:topDataProperty ;
            rdfs:domain cx-fx:Argument ;
            rdfs:range xsd:anyType;
            skos:example "a default string"^^xsd:string;
            skos:example <urn:default:uri>;
            skos:altLabel "Argument Default"@en;
            skos:prefLabel "Default"@en .

###  https://w3id.org/catenax/ontology/function#outputProperty
cx-fx:outputProperty rdf:type owl:DatatypeProperty ;
            rdfs:comment "Determines a path/name in the output response under which all output arguments are encoded. Default is '.'"@en;
            rdfs:subPropertyOf owl:topDataProperty ;
            rdfs:domain cx-fx:Result ;
            rdfs:range xsd:string;
            skos:example ".";
            skos:altLabel "Function Output Property"@en;
            skos:prefLabel "Output Property"@en .

###  https://w3id.org/catenax/ontology/function#resultIdProperty
cx-fx:resultIdProperty rdf:type owl:DatatypeProperty ;
            rdfs:comment "Determines a path in the output response under which the IRI of the result component will be transmitted."@en;
            rdfs:subPropertyOf owl:topDataProperty ;
            rdfs:domain cx-fx:Result ;
            rdfs:range xsd:string;
            skos:example "componentId";
            skos:altLabel "Function Result ID Property"@en;
            skos:prefLabel "Result ID Property"@en .

###  https://w3id.org/catenax/ontology/function#correlationInput
cx-fx:correlationInput rdf:type owl:ObjectProperty ;
            rdfs:comment "Correlates the <ttps://w3id.org/catenax/ontology/function#resultIdProperty> with a function argument."@en;
            rdfs:domain cx-fx:Result ;
            rdfs:range cx-fx:Argument;
            skos:altLabel "Function Correlation ID Inputy"@en;
            skos:prefLabel "Correlation ID Input"@en .

###  https://w3id.org/catenax/ontology/function#output
cx-fx:output rdf:type owl:ObjectProperty ;
            rdfs:domain cx-fx:Result ;
            rdfs:range cx-fx:ReturnValue;
            skos:altLabel "Function Return Output"@en;
            skos:prefLabel "Output"@en .

###  https://w3id.org/catenax/ontology/function#ReturnValue
cx-fx:ReturnValue rdf:type owl:Class ;
             rdfs:subClassOf cx-core:ConceptualObject ;
             skos:altLabel "Function Return Value Definition"@en ;
             skos:prefLabel "Return Value"@en .

###  https://w3id.org/catenax/ontology/function#valuePath
cx-fx:valuePath rdf:type owl:DatatypeProperty ;
            rdfs:comment "Determines a path in the output response under which a return value is transmitted."@en;
            rdfs:subPropertyOf owl:topDataProperty ;
            rdfs:domain cx-fx:ReturnValue ;
            rdfs:range xsd:string;
            skos:example "age";
            skos:altLabel "Function Result Value Path"@en;
            skos:prefLabel "Value Path"@en .

###  Generated by the OWL API (version 4.5.9.2019-02-01T07:24:44Z) https://github.com/owlcs/owlapi
